verify/InfiniteRect.v
@@ -1,0 +1,1055 @@
+From BusyCoq Require Import Individual62 LongN.
+Require Import Lia.
+Require Import List.
+Require Import PeanoNat.
+Require Import Bool.
+
+Module InfiniteRectInternal.
+
+Fixpoint sym_list_eqb (a b : list Sym) :=
+match a,b with
+| [], [] => true
+| x::xs, y::ys => if sym_eqb x y then sym_list_eqb xs ys else false
+| _, _ => false
+end.
+
+Lemma sym_list_eqb_spec a b:
+  Bool.reflect (a=b) (sym_list_eqb a b).
+Proof.
+  gen b.
+  induction a as [|x xs IH]; destruct b as [|y ys]; cbn.
+  - constructor.
+    reflexivity.
+  - constructor.
+    congruence.
+  - constructor.
+    congruence.
+  - destruct (sym_eqb_spec x y) as [Heq|Hneq].
+    + subst.
+      destruct (IH ys) as [Heq|Hneq].
+      * subst.
+        constructor.
+        reflexivity.
+      * constructor.
+        intro H.
+        inversion H; subst.
+        contradiction.
+    + constructor.
+      intro H.
+      inversion H; subst.
+      contradiction.
+Qed.
+
+Definition sideS_n tm (H : Stream (DH0*DH0)) (r : side) (n : nat) : Prop :=
+  exists k, sideRLs_n tm (Str_firstn k H) r n.
+
+Definition downRect tm (L R : Stream (DH0*DH0)) (w : list Sym) (width : nat) : Prop :=
+  forall r n,
+    sideS_n tm R r n ->
+    sideS_n tm L (w *> r) (width + n).
+
+Definition quadRect tm (L : Stream (DH0*DH0)) (top : side) : Prop :=
+  forall n, sideS_n tm L top n.
+
+Definition leftRealizes tm (h : DH0) (L : Stream (DH0*DH0)) (l : side) : Prop :=
+  forall k, exists ls h' l',
+    lcons h ls = (Str_firstn k L, h') /\
+    sideRLs (flip tm) ls l l'.
+
+Lemma Str_firstn_length {A} n (s : Stream A):
+  length (Str_firstn n s) = n.
+Proof.
+  gen s.
+  induction n; intros; cbn.
+  - reflexivity.
+  - rewrite IHn.
+    reflexivity.
+Qed.
+
+Lemma Str_firstn_add {A} n m (s : Stream A):
+  Str_firstn (n+m) s =
+  Str_firstn n s ++ Str_firstn m (Str_nth_tl n s).
+Proof.
+  gen s.
+  induction n; intros; cbn; trivial.
+  rewrite IHn.
+  reflexivity.
+Qed.
+
+Lemma Str_firstn_app {A} (xs : list A) (s : Stream A):
+  Str_firstn (length xs) (xs *> s) = xs.
+Proof.
+  induction xs; cbn.
+  - reflexivity.
+  - rewrite IHxs.
+    reflexivity.
+Qed.
+
+Lemma Str_firstn_app_add {A} (xs : list A) n (s : Stream A):
+  Str_firstn (length xs+n) (xs *> s) = xs ++ Str_firstn n s.
+Proof.
+  induction xs; cbn.
+  - reflexivity.
+  - rewrite IHxs.
+    reflexivity.
+Qed.
+
+Lemma Str_firstn_app_le {A} n (xs : list A) (s : Stream A):
+  n <= length xs ->
+  Str_firstn n (xs *> s) = firstn n xs.
+Proof.
+  gen xs.
+  induction n; intros xs Hle; cbn.
+  - reflexivity.
+  - destruct xs; cbn in *.
+    + lia.
+    + rewrite IHn by lia.
+      reflexivity.
+Qed.
+
+Lemma lcons_app h ls1 hs1 h1 ls2 hs2 h2:
+  lcons h ls1 = (hs1,h1) ->
+  lcons h1 ls2 = (hs2,h2) ->
+  lcons h (ls1++ls2) = (hs1++hs2,h2).
+Proof.
+  gen h hs1 h1.
+  induction ls1 as [|[a b] ls1 IH]; intros h hs1 h1 H1 H2; cbn in *.
+  - inversion H1; subst.
+    exact H2.
+  - destruct (lcons b ls1) as [hs0 h0] eqn:E.
+    inversion H1; subst.
+    rewrite (IH b hs0 h1 E H2).
+    reflexivity.
+Qed.
+
+Lemma lcons_firstn h ls hs h' k:
+  lcons h ls = (hs,h') ->
+  k <= length hs ->
+  exists h0, lcons h (firstn k ls) = (firstn k hs,h0).
+Proof.
+  gen h ls hs h'.
+  induction k; intros h ls hs h' H Hle.
+  - exists h.
+    reflexivity.
+  - destruct ls as [|[a b] ls].
+    + cbn in H.
+      inversion H; subst.
+      cbn in Hle.
+      lia.
+    + cbn in H.
+      destruct (lcons b ls) as [hs0 h0] eqn:E.
+      inversion H; subst.
+      cbn in Hle.
+      destruct (IHk b ls hs0 h' E) as [h1 H1]; [lia|].
+      exists h1.
+      cbn.
+      rewrite H1.
+      reflexivity.
+Qed.
+
+Lemma lcons_sideRLs_prefix tm h ls hs h' l l' k:
+  lcons h ls = (hs,h') ->
+  sideRLs tm ls l l' ->
+  k <= length hs ->
+  exists ls0 h0 l0,
+    lcons h ls0 = (firstn k hs,h0) /\
+    sideRLs tm ls0 l l0.
+Proof.
+  intros Hlcons Hside Hle.
+  destruct (lcons_firstn h ls hs h' k Hlcons Hle) as [h0 Hprefix].
+  pose proof (firstn_skipn k ls) as Hsplit.
+  rewrite <- Hsplit in Hside.
+  apply sideRLs_split in Hside.
+  destruct Hside as [l0 [Hside _]].
+  exists (firstn k ls), h0, l0.
+  split; assumption.
+Qed.
+
+Lemma sideRLs_n_prefix_extend tm H r n k1 k2:
+  k1 <= k2 ->
+  sideRLs_n tm (Str_firstn k1 H) r n ->
+  sideRLs_n tm (Str_firstn k2 H) r n.
+Proof.
+  intros Hle Hs.
+  replace k2 with (k1 + (k2-k1)) by lia.
+  rewrite Str_firstn_add.
+  eapply sideRLs_n_trans_1.
+  exact Hs.
+Qed.
+
+Lemma sideS_n_0 tm H r:
+  sideS_n tm H r O.
+Proof.
+  exists O.
+  cbn.
+  constructor.
+Qed.
+
+Lemma sideS_n_mono tm H r n m:
+  sideS_n tm H r n ->
+  m <= n ->
+  sideS_n tm H r m.
+Proof.
+  intros [k Hs] Hle.
+  exists k.
+  eapply sideRLs_n_mono; eauto.
+Qed.
+
+Lemma sideS_n_after tm H r n:
+  sideS_n tm H r n ->
+  forall k0, exists k,
+    k0 <= k /\
+    sideRLs_n tm (Str_firstn k H) r n.
+Proof.
+  intros [k Hs] k0.
+  exists (k + k0).
+  split.
+  - lia.
+  - eapply (sideRLs_n_prefix_extend tm H r n k (k+k0)); eauto; lia.
+Qed.
+
+Lemma sideS_n_app_split tm hs H r n:
+  sideS_n tm (hs *> H) r n ->
+  sideRLs_n tm hs r n \/
+  exists r', sideRLs tm hs r r' /\ sideS_n tm H r' n.
+Proof.
+  intros [k Hs].
+  destruct (Nat.leb_spec k (length hs)) as [Hle|Hgt].
+  - left.
+    eapply (sideRLs_n_prefix_extend tm (hs *> H) r n k (length hs)) in Hs; eauto.
+    rewrite Str_firstn_app in Hs.
+    exact Hs.
+  - replace k with (length hs+(k-length hs)) in Hs by lia.
+    rewrite Str_firstn_app_add in Hs.
+    apply sideRLs_n_split in Hs.
+    destruct Hs as [Hs|[r' [Hside Hs]]].
+    + left.
+      exact Hs.
+    + right.
+      exists r'.
+      split; [exact Hside|].
+      exists (k-length hs).
+      exact Hs.
+Qed.
+
+Lemma sideS_n_app_left tm hs H r n:
+  sideRLs_n tm hs r n ->
+  sideS_n tm (hs *> H) r n.
+Proof.
+  intros Hs.
+  exists (length hs).
+  rewrite Str_firstn_app.
+  exact Hs.
+Qed.
+
+Lemma sideS_n_app_right tm hs H r r' n:
+  sideRLs tm hs r r' ->
+  sideS_n tm H r' n ->
+  sideS_n tm (hs *> H) r n.
+Proof.
+  intros Hside [k Hs].
+  exists (length hs+k).
+  rewrite Str_firstn_app_add.
+  eapply sideRLs_n_trans_2; eauto.
+Qed.
+
+Lemma segRLs_to_segRLs_n_0 tm h1 h2 w1 w2:
+  segRLs tm h1 h2 w1 w2 ->
+  segRLs_n tm h1 h2 w1 w2 0.
+Proof.
+  intro H.
+  induction H; split; intros.
+  - inverts H.
+    constructor.
+  - eapply segRLs_sideRLs_concat; eauto.
+    constructor.
+  - cbn.
+    econstructor 1.
+    + intros l. apply H.
+    + destruct IHsegRLs as [IHn _].
+      apply IHn. exact H1.
+    + lia.
+  - eapply segRLs_sideRLs_concat; eauto.
+    econstructor; eauto.
+  - cbn.
+    eapply sideRLs_n_split in H3.
+    destruct H3 as [I1|[r2 [I1 I2]]].
+    + econstructor 2.
+      intros l.
+      specialize (H l r1).
+      apply with_counter in H.
+      destruct H as [n1 H].
+      eapply segLRs_sideRLs_n_concat in I1; eauto.
+      destruct I1 as [c [n2 [I2 I3]]].
+      do 3 eexists.
+      * eapply multistep_trans; eauto.
+      * lia.
+    + econstructor 1.
+      * intros l.
+        follow H.
+        eapply progress_evstep_trans.
+        2: apply H0.
+        eapply sideRLs_segLRs_concat; eauto.
+      * destruct IHsegRLs as [IHn _].
+        apply IHn. exact I2.
+      * lia.
+  - eapply segRLs_sideRLs_concat; eauto.
+    eapply segRLs_lrcons; eauto.
+Qed.
+
+Inductive segRLs_n1_tail tm:
+  list (DH0*DH0) -> list (DH0*DH0) -> list Sym -> list Sym -> Prop :=
+| segRLs_n1_tail_O w:
+    segRLs_n1_tail tm [] [] w w
+| segRLs_n1_tail_S ls1 ls2 w1 w2:
+    segRLs_n tm ls1 ls2 w1 w2 1 ->
+    segRLs_n1_tail tm ls1 ls2 w1 w2.
+
+Lemma segRLs_n_cons_segRL tm h1 h2 ls1 ls2 w1 w2 w3:
+  segRL tm h1 h2 w1 w2 ->
+  segRLs_n tm ls1 ls2 w2 w3 1 ->
+  segRLs_n tm ((h1,h2)::ls1) ls2 w1 w3 1.
+Proof.
+  unfold segRLs_n.
+  intros Hhead [Htail_n Htail].
+  split; intros.
+  - econstructor 1.
+    + intro l.
+      apply Hhead.
+    + apply Htail_n.
+      exact H.
+    + lia.
+  - econstructor.
+    + intro l.
+      apply Hhead.
+    + apply Htail.
+      exact H.
+Qed.
+
+Lemma segRLs_n_cons_tail tm h1 h2 ls1 ls2 w1 w2 w3:
+  segRL tm h1 h2 w1 w2 ->
+  segRLs_n1_tail tm ls1 ls2 w2 w3 ->
+  segRLs_n tm ((h1,h2)::ls1) ls2 w1 w3 1.
+Proof.
+  intros Hhead Htail.
+  inversion Htail; subst.
+  - apply segRLs_n_S.
+    exact Hhead.
+  - eapply segRLs_n_cons_segRL; eauto.
+Qed.
+
+Lemma lrcons_rcons h1 ls h2 h2' ls':
+  rcons ls h2 = (h2',ls') ->
+  (h1,h2')::ls' = lrcons h1 ls h2.
+Proof.
+  destruct ls as [|[a b] ls]; cbn; intros H.
+  - inversion H; reflexivity.
+  - inversion H; reflexivity.
+Qed.
+
+Definition segLLs_n1 tm h1 ls1 h2 ls2 w1 w2 :=
+  exists lsLR lsMid lsTail wLR wAfter hFinal,
+    ls2 = lsMid++lsTail /\
+    rcons lsLR hFinal = (h2,lsMid) /\
+    segLRs tm lsLR w1 wLR /\
+    segLL tm hFinal h1 wLR wAfter /\
+    segRLs_n1_tail tm ls1 lsTail wAfter w2.
+
+Lemma segRLs_n_lrcons_tail tm ls2 ls3 ls4 w1 w2 w3 w4 w5 h1 h2 h3 h4:
+  segRR' tm h1 h3 w1 w3 ->
+  segLL tm h4 h2 w4 w5 ->
+  segLRs tm ls2 w3 w4 ->
+  segRLs_n1_tail tm ls3 ls4 w5 w2 ->
+  segRLs_n tm ((h1,h2)::ls3) (lrcons h3 ls2 h4++ls4) w1 w2 1.
+Proof.
+  intros Hrr Hll Hlr Htail.
+  inversion Htail; subst.
+  - rewrite app_nil_r.
+    eapply segRLs_n_lrcons; eauto.
+  - change ((h1,h2)::ls3) with ([(h1,h2)]++ls3).
+    eapply (segRLs_n_trans tm [(h1,h2)] (lrcons h3 ls2 h4)
+      ls3 ls4 w1 w5 w2 1 1 1).
+    + eapply segRLs_n_lrcons; eauto.
+    + exact H.
+    + lia.
+    + lia.
+Qed.
+
+Lemma segRLs_n_RR_LLs tm ls3 ls4 w1 w2 w3 h1 h2 h3 h4:
+  segRR' tm h1 h3 w1 w3 ->
+  segLLs_n1 tm h2 ls3 h4 ls4 w3 w2 ->
+  segRLs_n tm ((h1,h2)::ls3) ((h3,h4)::ls4) w1 w2 1.
+Proof.
+  intros Hrr
+    (lsLR & lsMid & lsTail & wLR & wAfter & hFinal &
+      Hls4 & Hrcons & Hlr & Hll & Htail).
+  subst ls4.
+  change ((h3,h4)::lsMid++lsTail) with (((h3,h4)::lsMid)++lsTail).
+  rewrite (lrcons_rcons h3 lsLR hFinal h4 lsMid Hrcons).
+  eapply segRLs_n_lrcons_tail; eauto.
+Qed.
+
+Fixpoint segRLs_n1_c tm (ls1 ls2:list (DH0*DH0)) (w1 w2:list Sym) (T:nat) {struct T} :=
+match T with
+| O => false
+| S T =>
+match ls1 with
+| ((QR,qR),(QL,qL))::ls1 =>
+  match BoundedConfig.steps1 tm T (BoundedConfig.Build_T qR w1 QR R) with
+  | Some (BoundedConfig.Build_T l r q L, true) =>
+    match ls1, ls2 with
+    | [], [] =>
+      andb (sym_list_eqb r []) (andb (q_eqb q QL)
+      match skip_prefix_list qL l with
+      | Some w => sym_list_eqb w w2
+      | None => false
+      end)
+    | _::_, _ =>
+      andb (sym_list_eqb r []) (andb (q_eqb q QL)
+      match skip_prefix_list qL l with
+      | Some w => segRLs_n1_c tm ls1 ls2 w w2 T
+      | None => false
+      end)
+    | _, _ => false
+    end
+  | Some (BoundedConfig.Build_T l r q R, true) =>
+    match ls2 with
+    | ((QR',qR'),hL')::ls2 =>
+      andb (sym_list_eqb r []) (andb (q_eqb q QR')
+      match skip_prefix_list qR' l with
+      | Some w => segLLs_n1_c tm (QL,qL) ls1 hL' ls2 w w2 T
+      | None => false
+      end)
+    | [] => false
+    end
+  | _ => false
+  end
+| [] => false
+end
+end
+with segLLs_n1_c tm h1 ls1 h2 ls2 w1 w2 T {struct T} :=
+match T with
+| O => false
+| S T =>
+let '(QL,qL) := h2 in
+match BoundedConfig.steps1 tm T (BoundedConfig.Build_T qL w1 QL L) with
+| Some (BoundedConfig.Build_T l r q R, flag) =>
+  match ls2 with
+  | ((QR',qR'),hL')::ls2 =>
+    andb (sym_list_eqb r []) (andb (q_eqb q QR')
+    match skip_prefix_list qR' l with
+    | Some w => segLLs_n1_c tm h1 ls1 hL' ls2 w w2 T
+    | None => false
+    end)
+  | [] => false
+  end
+| Some (BoundedConfig.Build_T l r q L, flag) =>
+  let '(QL0,qL0) := h1 in
+  andb (sym_list_eqb r []) (andb (q_eqb q QL0)
+  match skip_prefix_list qL0 l with
+  | Some w =>
+    match ls1, ls2 with
+    | [], [] => sym_list_eqb w w2
+    | [], _ => false
+    | _::_, _ => segRLs_n1_c tm ls1 ls2 w w2 T
+    end
+  | None => false
+  end)
+| _ => false
+end
+end.
+
+Ltac split_andb H :=
+  repeat match type of H with
+  | andb _ _ = true =>
+    let Ha := fresh "H" in
+    apply andb_true_iff in H as [Ha H]
+  end.
+
+Lemma segRLs_LLs_n1_c_spec tm T:
+  (forall ls1 ls2 w1 w2,
+    segRLs_n1_c tm ls1 ls2 w1 w2 T = true ->
+    segRLs_n tm ls1 ls2 w1 w2 1) /\
+  (forall h1 ls1 h2 ls2 w1 w2,
+    segLLs_n1_c tm h1 ls1 h2 ls2 w1 w2 T = true ->
+    segLLs_n1 tm h1 ls1 h2 ls2 w1 w2).
+Proof.
+  induction T as [|T IH]; cbn [segRLs_n1_c segLLs_n1_c]; split; intros; try congruence.
+  - destruct IH as [IHseg IHll].
+    destruct ls1 as [|[[QR qR] [QL qL]] ls1]; cbn in H; [congruence|].
+    pose proof (BoundedConfig.steps1_spec tm T
+      (BoundedConfig.Build_T qR w1 QR R)) as Hstep.
+    destruct (BoundedConfig.steps1 tm T
+      (BoundedConfig.Build_T qR w1 QR R)) as [[x flag]|] eqn:Estep;
+      [|congruence].
+    destruct x as [l r q d].
+    destruct d; destruct flag; cbn in H; try congruence.
+    + destruct ls1 as [|p ls1'].
+      * destruct ls2 as [|p ls2']; cbn in H; [|congruence].
+        split_andb H.
+        destruct (sym_list_eqb_spec r []); [subst|congruence].
+        destruct (q_eqb_spec q QL); [subst|congruence].
+        destruct (skip_prefix_list qL l) as [w|] eqn:ESkip; cbn in H;
+          [|congruence].
+        apply skip_prefix_list_spec in ESkip.
+        assert (Hfirst: segRL tm (QR,qR) (QL,qL) w1 w).
+        {
+          unfold segRL.
+          intros l0 r0.
+          specialize (Hstep l0 r0).
+          cbn in Hstep.
+          rewrite ESkip in Hstep.
+          rewrite Str_app_assoc in Hstep.
+          exact Hstep.
+        }
+        destruct (sym_list_eqb_spec w w2); [subst|congruence].
+        eapply segRLs_n_cons_tail.
+        -- exact Hfirst.
+        -- constructor.
+      * split_andb H.
+        destruct (sym_list_eqb_spec r []); [subst|congruence].
+        destruct (q_eqb_spec q QL); [subst|congruence].
+        destruct (skip_prefix_list qL l) as [w|] eqn:ESkip; cbn in H;
+          [|congruence].
+        apply skip_prefix_list_spec in ESkip.
+        assert (Hfirst: segRL tm (QR,qR) (QL,qL) w1 w).
+        {
+          unfold segRL.
+          intros l0 r0.
+          specialize (Hstep l0 r0).
+          cbn in Hstep.
+          rewrite ESkip in Hstep.
+          rewrite Str_app_assoc in Hstep.
+          exact Hstep.
+        }
+        eapply segRLs_n_cons_tail.
+        -- exact Hfirst.
+        -- constructor.
+           eapply IHseg.
+           exact H.
+    + destruct ls2 as [|[[QR' qR'] hL'] ls2]; cbn in H; [congruence|].
+      split_andb H.
+      destruct (sym_list_eqb_spec r []); [subst|congruence].
+      destruct (q_eqb_spec q QR'); [subst|congruence].
+      destruct (skip_prefix_list qR' l) as [w|] eqn:ESkip; cbn in H;
+        [|congruence].
+      apply skip_prefix_list_spec in ESkip.
+      eapply segRLs_n_RR_LLs.
+      * unfold segRR'.
+        intros l0 r0.
+        specialize (Hstep l0 r0).
+        cbn in Hstep.
+        rewrite ESkip in Hstep.
+        rewrite Str_app_assoc in Hstep.
+        exact Hstep.
+      * eapply IHll.
+        exact H.
+  - destruct IH as [IHseg IHll].
+    destruct h2 as [QL qL].
+    pose proof (BoundedConfig.steps1_spec tm T
+      (BoundedConfig.Build_T qL w1 QL L)) as Hstep.
+    destruct (BoundedConfig.steps1 tm T
+      (BoundedConfig.Build_T qL w1 QL L)) as [[x flag]|] eqn:Estep;
+      [|congruence].
+    destruct x as [l r q d].
+    destruct d; cbn in H.
+    + destruct h1 as [QL0 qL0].
+      split_andb H.
+      destruct (sym_list_eqb_spec r []); [subst|congruence].
+      destruct (q_eqb_spec q QL0); [subst|congruence].
+      destruct (skip_prefix_list qL0 l) as [w|] eqn:ESkip; cbn in H;
+        [|congruence].
+      apply skip_prefix_list_spec in ESkip.
+      assert (Hll: segLL tm (QL,qL) (QL0,qL0) w1 w).
+      {
+        unfold segLL.
+        intros l0 r0.
+        destruct flag.
+        - apply progress_evstep.
+          specialize (Hstep l0 r0).
+          cbn in Hstep.
+          rewrite ESkip in Hstep.
+          rewrite Str_app_assoc in Hstep.
+          exact Hstep.
+        - specialize (Hstep l0 r0).
+          cbn in Hstep.
+          rewrite ESkip in Hstep.
+          rewrite Str_app_assoc in Hstep.
+          exact Hstep.
+      }
+      destruct ls1 as [|p ls1'].
+      * destruct ls2 as [|p ls2']; cbn in H; [|congruence].
+        destruct (sym_list_eqb_spec w w2); [subst|congruence].
+        exists (@nil (DH0*DH0)), (@nil (DH0*DH0)), (@nil (DH0*DH0)),
+          w1, w2, (QL,qL).
+        repeat split.
+        -- constructor.
+        -- exact Hll.
+        -- constructor.
+      * exists (@nil (DH0*DH0)), (@nil (DH0*DH0)), ls2, w1, w, (QL,qL).
+        repeat split.
+        -- constructor.
+        -- exact Hll.
+        -- constructor.
+           eapply IHseg.
+           exact H.
+    + destruct ls2 as [|[[QR' qR'] hL'] ls2]; cbn in H; [congruence|].
+      split_andb H.
+      destruct (sym_list_eqb_spec r []); [subst|congruence].
+      destruct (q_eqb_spec q QR'); [subst|congruence].
+      destruct (skip_prefix_list qR' l) as [w|] eqn:ESkip; cbn in H;
+        [|congruence].
+      apply skip_prefix_list_spec in ESkip.
+      assert (Hlr: segLR tm (QL,qL) (QR',qR') w1 w).
+      {
+        unfold segLR.
+        intros l0 r0.
+        destruct flag.
+        - specialize (Hstep l0 r0).
+          cbn in Hstep.
+          rewrite ESkip in Hstep.
+          rewrite Str_app_assoc in Hstep.
+          eapply progress_evstep.
+          exact Hstep.
+        - specialize (Hstep l0 r0).
+          cbn in Hstep.
+          rewrite ESkip in Hstep.
+          rewrite Str_app_assoc in Hstep.
+          exact Hstep.
+      }
+      destruct (IHll h1 ls1 hL' ls2 w w2 H)
+        as (lsLR & lsMid & lsTail & wLR & wAfter & hFinal &
+          Hls2 & Hrcons & HlrTail & Hll & Htail).
+      subst ls2.
+      exists (((QL,qL),(QR',qR'))::lsLR),
+        (((QR',qR'),hL')::lsMid), lsTail, wLR, wAfter, hFinal.
+      repeat split; eauto.
+      * cbn.
+        rewrite <- (lrcons_rcons (QR',qR') lsLR hFinal hL' lsMid Hrcons).
+        reflexivity.
+      * econstructor; eauto.
+Qed.
+
+Lemma segRLs_n1_c_spec tm ls1 ls2 w1 w2 T:
+  segRLs_n1_c tm ls1 ls2 w1 w2 T = true ->
+  segRLs_n tm ls1 ls2 w1 w2 1.
+Proof.
+  pose proof (segRLs_LLs_n1_c_spec tm T) as [Hspec _].
+  apply Hspec.
+Qed.
+
+Lemma downRect_concat tm L M R w1 w2 width1 width2:
+  downRect tm L M w1 width1 ->
+  downRect tm M R w2 width2 ->
+  downRect tm L R (w1++w2) (width1+width2).
+Proof.
+  unfold downRect.
+  intros H1 H2 r n HR.
+  specialize (H2 r n HR).
+  specialize (H1 (w2 *> r) (width2+n) H2).
+  replace ((width1 + width2) + n) with (width1 + (width2+n)) by lia.
+  rewrite Str_app_assoc.
+  exact H1.
+Qed.
+
+Lemma downRect_quadRect_concat tm L R w width top:
+  downRect tm L R w width ->
+  quadRect tm R top ->
+  quadRect tm L (w *> top).
+Proof.
+  unfold quadRect.
+  intros Hrect Hquad n.
+  eapply sideS_n_mono with (n:=width+n).
+  - apply Hrect.
+    apply Hquad.
+  - lia.
+Qed.
+
+Lemma segRLs_n_downRect_trans tm hL hR L R w1 w2 width:
+  segRLs_n tm hL hR w1 w2 width ->
+  downRect tm L R w2 width ->
+  downRect tm (hL *> L) (hR *> R) w1 width.
+Proof.
+  unfold downRect.
+  intros [Hseg_n Hseg] Hrect r n HR.
+  destruct (sideS_n_app_split tm hR R r n HR) as [HR'|[r' [Hside HR']]].
+  - apply sideS_n_app_left.
+    apply Hseg_n.
+    exact HR'.
+  - eapply sideS_n_app_right.
+    + apply Hseg.
+      exact Hside.
+    + apply Hrect.
+      exact HR'.
+Qed.
+
+Lemma downRect_width_mono tm L R w width width':
+  downRect tm L R w width ->
+  width' <= width ->
+  downRect tm L R w width'.
+Proof.
+  unfold downRect.
+  intros H Hle r n HR.
+  eapply sideS_n_mono.
+  - apply H. exact HR.
+  - lia.
+Qed.
+
+Lemma downRect_of_segRLs_n tm L R w width
+  (I : Type) (KL KR : I -> nat) (bot : I -> list Sym):
+  (forall kR0, exists i,
+    kR0 <= KR i /\
+    segRLs_n tm
+      (Str_firstn (KL i) L)
+      (Str_firstn (KR i) R)
+      w (bot i) width) ->
+  downRect tm L R w width.
+Proof.
+  unfold downRect, sideS_n.
+  intros Hrect r n [kR HR].
+  destruct (Hrect kR) as [i [Hle Hseg]].
+  exists (KL i).
+  destruct Hseg as [Hseg _].
+  apply Hseg.
+  eapply sideRLs_n_prefix_extend; eauto.
+Qed.
+
+Lemma downRect_segRLs_progress_iter tm width
+  (P : Stream (DH0*DH0) -> Stream (DH0*DH0) -> list Sym -> Prop):
+  (forall L R top, P L R top -> exists hL hR bot L' R',
+    O < length hR /\
+    L = hL *> L' /\
+    R = hR *> R' /\
+    segRLs_n tm hL hR top bot width /\
+    P L' R' bot) ->
+  forall n L R top,
+    P L R top ->
+    exists hL hR bot L' R',
+      n <= length hR /\
+      L = hL *> L' /\
+      R = hR *> R' /\
+      segRLs_n tm hL hR top bot width /\
+      P L' R' bot.
+Proof.
+  intros Hprog.
+  induction n; intros L R top HP.
+  - destruct (Hprog L R top HP) as [hL [hR [bot [L' [R' [Hlen [HL [HR [Hseg HP']]]]]]]]].
+    exists hL, hR, bot, L', R'.
+    split; [lia|].
+    split; [exact HL|].
+    split; [exact HR|].
+    split; [exact Hseg|exact HP'].
+  - destruct (Hprog L R top HP) as [hL1 [hR1 [mid [L1 [R1 [Hlen1 [HL1 [HR1 [Hseg1 HP1]]]]]]]]].
+    destruct (IHn L1 R1 mid HP1)
+      as [hL2 [hR2 [bot [L2 [R2 [Hle [HL2 [HR2 [Hseg2 HP2]]]]]]]]].
+    exists (hL1++hL2), (hR1++hR2), bot, L2, R2.
+    split; [rewrite length_app; lia|].
+    split.
+    + rewrite HL1, HL2, Str_app_assoc.
+      reflexivity.
+    + split.
+      * rewrite HR1, HR2, Str_app_assoc.
+        reflexivity.
+      * split.
+        -- eapply segRLs_n_trans; eauto; lia.
+        -- exact HP2.
+Qed.
+
+Lemma segRLs_n_inf_trans tm L R w width
+  (P : Stream (DH0*DH0) -> Stream (DH0*DH0) -> list Sym -> Prop):
+  (forall L0 R0 top, P L0 R0 top -> exists hL hR bot L' R',
+    O < length hR /\
+    L0 = hL *> L' /\
+    R0 = hR *> R' /\
+    segRLs_n tm hL hR top bot width /\
+    P L' R' bot) ->
+  P L R w ->
+  downRect tm L R w width.
+Proof.
+  unfold downRect, sideS_n.
+  intros Hprog HP0 r n [kR HR].
+  destruct (downRect_segRLs_progress_iter tm width P Hprog kR L R w HP0)
+    as [hL [hR [bot [L' [R' [Hle [HL [HR' [Hseg _]]]]]]]]].
+  exists (length hL).
+  rewrite HL.
+  rewrite Str_firstn_app.
+  destruct Hseg as [Hseg _].
+  apply Hseg.
+  assert (Hside: sideRLs_n tm (Str_firstn (length hR) R) r n).
+  {
+    eapply sideRLs_n_prefix_extend; eauto.
+  }
+  rewrite HR' in Hside.
+  rewrite Str_firstn_app in Hside.
+  exact Hside.
+Qed.
+
+Lemma leftRealizes_progress_iter tm
+  (P : DH0 -> Stream (DH0*DH0) -> side -> Prop):
+  (forall h L l, P h L l -> exists hs L' h' ls l',
+    O < length hs /\
+    L = hs *> L' /\
+    lcons h ls = (hs,h') /\
+    sideRLs (flip tm) ls l l' /\
+    P h' L' l') ->
+  forall n h L l,
+    P h L l ->
+    exists hs L' h' ls l',
+      n <= length hs /\
+      L = hs *> L' /\
+      lcons h ls = (hs,h') /\
+      sideRLs (flip tm) ls l l' /\
+      P h' L' l'.
+Proof.
+  intros Hprog.
+  induction n; intros h L l HP.
+  - destruct (Hprog h L l HP) as [hs [L' [h' [ls [l' [Hlen [HL [Hlcons [Hside HP']]]]]]]]].
+    exists hs, L', h', ls, l'.
+    split; [lia|].
+    split; [exact HL|].
+    split; [exact Hlcons|].
+    split; [exact Hside|exact HP'].
+  - destruct (Hprog h L l HP) as [hs1 [L1 [h1 [ls1 [l1 [Hlen1 [HL1 [Hlcons1 [Hside1 HP1]]]]]]]]].
+    destruct (IHn h1 L1 l1 HP1)
+      as [hs2 [L2 [h2 [ls2 [l2 [Hle [HL2 [Hlcons2 [Hside2 HP2]]]]]]]]].
+    exists (hs1++hs2), L2, h2, (ls1++ls2), l2.
+    split; [rewrite length_app; lia|].
+    split.
+    + rewrite HL1, HL2, Str_app_assoc.
+      reflexivity.
+    + split.
+      * eapply lcons_app; eauto.
+      * split.
+        -- eapply sideRLs_trans; eauto.
+        -- exact HP2.
+Qed.
+
+Lemma leftRealizes_inf_concat tm h L l
+  (P : DH0 -> Stream (DH0*DH0) -> side -> Prop):
+  (forall h0 L0 l0, P h0 L0 l0 -> exists hs L' h' ls l',
+    O < length hs /\
+    L0 = hs *> L' /\
+    lcons h0 ls = (hs,h') /\
+    sideRLs (flip tm) ls l0 l' /\
+    P h' L' l') ->
+  P h L l ->
+  leftRealizes tm h L l.
+Proof.
+  unfold leftRealizes.
+  intros Hprog HP k.
+  destruct (leftRealizes_progress_iter tm P Hprog k h L l HP)
+    as [hs [L' [h' [ls [l' [Hle [HL [Hlcons [Hside _]]]]]]]]].
+  destruct (lcons_sideRLs_prefix (flip tm) h ls hs h' l l' k Hlcons Hside Hle)
+    as [ls0 [h0 [l0 [Hlcons0 Hside0]]]].
+  exists ls0, h0, l0.
+  split.
+  - rewrite HL.
+    rewrite Str_firstn_app_le by exact Hle.
+    exact Hlcons0.
+  - exact Hside0.
+Qed.
+
+Lemma sideRLs_leftRealizes_trans tm h hs L l h' ls l':
+  lcons h ls = (hs,h') ->
+  sideRLs (flip tm) ls l l' ->
+  leftRealizes tm h' L l' ->
+  leftRealizes tm h (hs *> L) l.
+Proof.
+  unfold leftRealizes.
+  intros Hlcons Hside Htail k.
+  destruct (Nat.leb_spec k (length hs)) as [Hle|Hgt].
+  - destruct (lcons_sideRLs_prefix (flip tm) h ls hs h' l l' k
+      Hlcons Hside Hle) as [ls0 [h0 [l0 [Hlcons0 Hside0]]]].
+    exists ls0, h0, l0.
+    split.
+    + rewrite Str_firstn_app_le by exact Hle.
+      exact Hlcons0.
+    + exact Hside0.
+  - destruct (Htail (k-length hs)) as [ls0 [h0 [l0 [Hlcons0 Hside0]]]].
+    exists (ls++ls0), h0, l0.
+    split.
+    + rewrite (lcons_app h ls hs h' ls0 (Str_firstn (k-length hs) L) h0
+        Hlcons Hlcons0).
+      replace k with (length hs+(k-length hs)) by lia.
+      rewrite Str_firstn_app_add.
+      replace (length hs + (k - length hs) - length hs)
+        with (k-length hs) by lia.
+      reflexivity.
+    + eapply sideRLs_trans; eauto.
+Qed.
+
+Lemma downRect_inf_concat tm L top
+  (P : Stream (DH0*DH0) -> side -> Prop):
+  (forall L0 top0, P L0 top0 -> exists L' top' w width,
+    O < width /\
+    top0 = w *> top' /\
+    downRect tm L0 L' w width /\
+    P L' top') ->
+  P L top ->
+  quadRect tm L top.
+Proof.
+  intros Hstep.
+  assert (H: forall n L0 top0, P L0 top0 -> sideS_n tm L0 top0 n).
+  {
+    induction n; intros L0 top0 HP.
+    - apply sideS_n_0.
+    - destruct (Hstep L0 top0 HP) as [L' [top' [w [width [Hwidth [HT [Hrect HP']]]]]]].
+      rewrite HT.
+      eapply sideS_n_mono.
+      + apply Hrect.
+        apply IHn.
+        exact HP'.
+      + lia.
+  }
+  intros HP n.
+  apply H.
+  exact HP.
+Qed.
+
+Lemma quadRect_runs tm L top h l:
+  quadRect tm L top ->
+  leftRealizes tm h L l ->
+  forall n, exists c,
+    l {{{ (h,R) }}} top -[ tm ]->> n / c.
+Proof.
+  intros Hrect Hleft n.
+  destruct (sideS_n_after tm L top n (Hrect n) n) as [k [Hnk Hside]].
+  destruct (Hleft k) as [ls [h' [l' [Hlcons Hflip]]]].
+  eapply sideRLs_n_sideRLs_concat in Hside.
+  4: exact Hflip.
+  2: exact Hlcons.
+  2: rewrite Str_firstn_length; exact Hnk.
+  exact Hside.
+Qed.
+
+Lemma quadRect_nonhalt tm L top h l:
+  quadRect tm L top ->
+  leftRealizes tm h L l ->
+  ~halts tm (l {{{ (h,R) }}} top).
+Proof.
+  intros Hrect Hleft.
+  apply step_unbounded_nonhalt.
+  apply (quadRect_runs tm L top h l); assumption.
+Qed.
+
+Lemma progress_rect_nonhalt_cond tm L top
+  (P : Stream (DH0*DH0) -> side -> Prop) h l:
+  (forall L0 top0, P L0 top0 -> exists L' top' w width,
+    O < width /\
+    top0 = w *> top' /\
+    downRect tm L0 L' w width /\
+    P L' top') ->
+  P L top ->
+  leftRealizes tm h L l ->
+  ~halts tm (l {{{ (h,R) }}} top).
+Proof.
+  intros Hstep HP Hleft.
+  eapply quadRect_nonhalt.
+  - eapply downRect_inf_concat; eauto.
+  - exact Hleft.
+Qed.
+
+Arguments sideS_n {tm} H r n.
+
+End InfiniteRectInternal.
+
+Definition downRect tm (L R : Stream (DH0*DH0)) (w : list Sym) (width : nat) :=
+  @InfiniteRectInternal.downRect tm L R w width.
+Definition quadRect tm (L : Stream (DH0*DH0)) (top : side) :=
+  @InfiniteRectInternal.quadRect tm L top.
+Definition leftRealizes tm (h : DH0) (L : Stream (DH0*DH0)) (l : side) :=
+  @InfiniteRectInternal.leftRealizes tm h L l.
+Definition segRLs_n1_c tm (ls1 ls2:list (DH0*DH0)) (w1 w2:list Sym) (T:nat) :=
+  @InfiniteRectInternal.segRLs_n1_c tm ls1 ls2 w1 w2 T.
+
+Lemma segRLs_n1_c_spec tm ls1 ls2 w1 w2 T:
+  segRLs_n1_c tm ls1 ls2 w1 w2 T = true ->
+  segRLs_n tm ls1 ls2 w1 w2 1.
+Proof.
+  exact (InfiniteRectInternal.segRLs_n1_c_spec tm ls1 ls2 w1 w2 T).
+Qed.
+
+Ltac solve_segRLs_n1_with bound :=
+  eapply (segRLs_n1_c_spec _ _ _ _ _ bound); vm_compute; reflexivity.
+
+Ltac solve_segRLs_n1 :=
+  first [
+    let bound := constr:(1000) in solve_segRLs_n1_with bound
+  | solve_segRLs_n
+  ].
+
+Lemma segRLs_n_downRect_trans tm hL hR L R w1 w2 width:
+  segRLs_n tm hL hR w1 w2 width ->
+  downRect tm L R w2 width ->
+  downRect tm (hL *> L) (hR *> R) w1 width.
+Proof.
+  exact (InfiniteRectInternal.segRLs_n_downRect_trans tm hL hR L R w1 w2 width).
+Qed.
+
+Lemma segRLs_n_inf_trans tm L R w width
+  (P : Stream (DH0*DH0) -> Stream (DH0*DH0) -> list Sym -> Prop):
+  (forall L0 R0 top, P L0 R0 top -> exists hL hR bot L' R',
+    O < length hR /\
+    L0 = hL *> L' /\
+    R0 = hR *> R' /\
+    segRLs_n tm hL hR top bot width /\
+    P L' R' bot) ->
+  P L R w ->
+  downRect tm L R w width.
+Proof.
+  exact (InfiniteRectInternal.segRLs_n_inf_trans tm L R w width P).
+Qed.
+
+Lemma downRect_quadRect_concat tm L R w width top:
+  downRect tm L R w width ->
+  quadRect tm R top ->
+  quadRect tm L (w *> top).
+Proof.
+  exact (InfiniteRectInternal.downRect_quadRect_concat tm L R w width top).
+Qed.
+
+Lemma downRect_inf_concat tm L top
+  (P : Stream (DH0*DH0) -> side -> Prop):
+  (forall L0 top0, P L0 top0 -> exists L' top' w width,
+    O < width /\
+    top0 = w *> top' /\
+    downRect tm L0 L' w width /\
+    P L' top') ->
+  P L top ->
+  quadRect tm L top.
+Proof.
+  exact (InfiniteRectInternal.downRect_inf_concat tm L top P).
+Qed.
+
+Lemma leftRealizes_inf_concat tm h L l
+  (P : DH0 -> Stream (DH0*DH0) -> side -> Prop):
+  (forall h0 L0 l0, P h0 L0 l0 -> exists hs L' h' ls l',
+    O < length hs /\
+    L0 = hs *> L' /\
+    lcons h0 ls = (hs,h') /\
+    sideRLs (flip tm) ls l0 l' /\
+    P h' L' l') ->
+  P h L l ->
+  leftRealizes tm h L l.
+Proof.
+  exact (InfiniteRectInternal.leftRealizes_inf_concat tm h L l P).
+Qed.
+
+Lemma sideRLs_leftRealizes_trans tm h hs L l h' ls l':
+  lcons h ls = (hs,h') ->
+  sideRLs (flip tm) ls l l' ->
+  leftRealizes tm h' L l' ->
+  leftRealizes tm h (hs *> L) l.
+Proof.
+  exact (InfiniteRectInternal.sideRLs_leftRealizes_trans tm h hs L l h' ls l').
+Qed.
+
+Lemma quadRect_nonhalt tm L top h l:
+  quadRect tm L top ->
+  leftRealizes tm h L l ->
+  ~halts tm (l {{{ (h,R) }}} top).
+Proof.
+  exact (InfiniteRectInternal.quadRect_nonhalt tm L top h l).
+Qed.
+
+Opaque downRect quadRect leftRealizes.
