verify/InfiniteRect_v1.v
@@ -1,0 +1,943 @@
+From BusyCoq Require Import Individual62 InfiniteRect LongN.
+Require Import Bool.
+Require Import List.
+Require Import Lia.
+Require Import PeanoNat.
+Require Import String.
+Require Import ZifyNat.
+
+Open Scope list.
+Close Scope sym_scope.
+
+Module TM4.
+
+Definition tm := Eval compute in (TM_from_str "1LB0RA_0LC0LB_1RD0LF_1RD0RE_1LA1RE_---1LE").
+
+Inductive Tok :=
+| RTok (q : Q)
+| LTok (q : Q).
+
+Definition tok_eqb a b :=
+  match a,b with
+  | RTok q1, RTok q2 => q_eqb q1 q2
+  | LTok q1, LTok q2 => q_eqb q1 q2
+  | _, _ => false
+  end.
+
+Record Boundary := {
+  b_mu : nat;
+  b_p : nat;
+  b_pre : list Tok;
+  b_per : list Tok;
+}.
+
+Definition tok_default := RTok A.
+
+Definition tok_at (b : Boundary) n :=
+  if n <? b.(b_mu) then
+    nth n b.(b_pre) tok_default
+  else
+    nth ((n - b.(b_mu)) mod b.(b_p)) b.(b_per) tok_default.
+
+Fixpoint write_sym n s xs :=
+  match n,xs with
+  | O, [] => [s]
+  | O, _::xs => s::xs
+  | S n, [] => S0::write_sym n s []
+  | S n, x::xs => x::write_sym n s xs
+  end.
+
+Record RunState := {
+  rs_left : nat;
+  rs_q : Q;
+  rs_pos : nat;
+  rs_tape : list Sym;
+  rs_out : list Tok;
+}.
+
+Definition finish_or_continue need (st : RunState) tok :=
+  let out := tok :: st.(rs_out) in
+  if need <=? List.length out then
+    Some (inr (rev out))
+  else
+    Some (inl {|
+      rs_left := st.(rs_left);
+      rs_q := st.(rs_q);
+      rs_pos := st.(rs_pos);
+      rs_tape := st.(rs_tape);
+      rs_out := out;
+    |}).
+
+Definition run_step (b : Boundary) need (st : RunState) :=
+  let s := nth st.(rs_pos) st.(rs_tape) S0 in
+  match tm (st.(rs_q), s) with
+  | None => None
+  | Some (s', d, q') =>
+      let tape' := write_sym st.(rs_pos) s' st.(rs_tape) in
+      match d with
+      | R =>
+          let st' := {|
+            rs_left := st.(rs_left);
+            rs_q := q';
+            rs_pos := S st.(rs_pos);
+            rs_tape := tape';
+            rs_out := st.(rs_out);
+          |} in
+          match st.(rs_pos) with
+          | O => finish_or_continue need st' (RTok q')
+          | S _ => Some (inl st')
+          end
+      | L =>
+          match st.(rs_pos) with
+          | O =>
+              if tok_eqb (LTok q') (tok_at b st.(rs_left)) then
+                match tok_at b (S st.(rs_left)) with
+                | RTok qin =>
+                    Some (inl {|
+                      rs_left := st.(rs_left) + 2;
+                      rs_q := qin;
+                      rs_pos := O;
+                      rs_tape := tape';
+                      rs_out := st.(rs_out);
+                    |})
+                | LTok _ => None
+                end
+              else None
+          | S pos' =>
+              let st' := {|
+                rs_left := st.(rs_left);
+                rs_q := q';
+                rs_pos := pos';
+                rs_tape := tape';
+                rs_out := st.(rs_out);
+              |} in
+              match pos' with
+              | O => finish_or_continue need st' (LTok q')
+              | S _ => Some (inl st')
+              end
+          end
+      end
+  end.
+
+Fixpoint run_until fuel (b : Boundary) need (st : RunState) :=
+  if need <=? List.length st.(rs_out) then Some (rev st.(rs_out)) else
+  match fuel with
+  | O => None
+  | S fuel =>
+      match run_step b need st with
+      | Some (inl st') => run_until fuel b need st'
+      | Some (inr out) => Some out
+      | None => None
+      end
+  end.
+
+Definition initial_state (b : Boundary) :=
+  match tok_at b O with
+  | RTok q => Some {|
+      rs_left := 1;
+      rs_q := q;
+      rs_pos := O;
+      rs_tape := [];
+      rs_out := [];
+    |}
+  | LTok _ => None
+  end.
+
+Definition gen_fuel need := 1000 + 50 * (need + 10).
+
+Definition empty_boundary mu p := {|
+  b_mu := mu;
+  b_p := p;
+  b_pre := [];
+  b_per := [];
+|}.
+
+Definition gen_next (b : Boundary) mu p :=
+  let need := mu + p in
+  match initial_state b with
+  | Some st =>
+      match run_until (gen_fuel need) b need st with
+      | Some out => {|
+          b_mu := mu;
+          b_p := p;
+          b_pre := firstn mu out;
+          b_per := firstn p (skipn mu out);
+        |}
+      | None => empty_boundary mu p
+      end
+  | None => empty_boundary mu p
+  end.
+
+Definition B0_pre :=
+  [RTok E; LTok A; RTok E; LTok B; RTok E; LTok A; RTok E; LTok B;
+   RTok E; LTok A; RTok E; LTok B; RTok E; LTok A; RTok E; LTok E].
+
+Definition B0_per :=
+  [RTok A; LTok C; RTok D; LTok B; RTok E; LTok A].
+
+Definition B0 := {|
+  b_mu := 16;
+  b_p := 6;
+  b_pre := B0_pre;
+  b_per := B0_per;
+|}.
+
+Definition len_table : list (nat*nat) :=
+  [(16,6); (24,18); (18,22); (18,20); (14,26); (22,18); (18,4); (14,6);
+   (10,18); (10,22); (6792,20); (8834,26); (6122,18); (4172,4); (6248,6); (4678,18);
+   (5722,22); (5206,20); (6724,26); (4660,18); (3226,4); (4794,6); (3606,18); (4378,22);
+   (3966,20); (5124,26); (3552,18); (2408,4); (3540,6); (2674,18); (3240,22); (2948,20);
+   (3744,26); (2630,18); (1866,4); (2616,6); (2024,18); (2348,22); (2434,20); (3130,26);
+   (2200,18); (1576,4); (2178,6); (1678,18); (2024,22); (1880,20); (2354,26); (1684,18);
+   (1228,4); (1714,6); (1344,18); (1516,22); (1386,20); (1712,26); (1242,18); (944,4);
+   (1212,6); (932,18); (1080,22); (974,20); (1176,26); (868,18); (688,4); (860,6);
+   (698,18); (758,22); (1034,20); (1270,26); (920,18); (710,4); (910,6); (756,18);
+   (844,22); (750,20); (888,26); (670,18); (550,4); (676,6); (554,18); (600,22);
+   (522,20); (628,26); (450,18); (382,4); (448,6); (376,18); (414,22); (482,20);
+   (574,26); (416,18); (346,4); (404,6); (324,18); (338,22); (286,20); (332,26);
+   (262,18); (264,4); (270,6); (226,18); (222,22); (200,20); (252,26); (202,18);
+   (176,4); (162,6); (148,18); (140,22); (124,20); (114,26); (84,18); (98,4);
+   (84,6); (82,18); (82,22); (80,20); (70,26); (62,18); (62,4); (74,6);
+   (62,18); (70,22); (62,20); (48,26); (52,18); (46,4); (52,6); (50,18);
+   (48,22); (40,20); (32,26); (28,18); (40,4); (42,6); (32,18); (38,22);
+   (24,20); (16,26); (20,18); (14,4); (18,6); (22,18); (20,22); (20,20);
+   (14,26); (18,18); (12,4); (10,6); (10,18); (6,22); (2,20); (O,26);
+   (O,18); (16,4); (24,6); (18,18); (20,22); (12,20); (8,26); (8,18);
+   (10,4)].
+
+Definition len_at i := nth i len_table (O,2).
+
+Fixpoint build_boundaries_from i n b :=
+  match n with
+  | O => [b]
+  | S n =>
+      let '(mu,p) := len_at (S i) in
+      let b' := gen_next b mu p in
+      b :: build_boundaries_from (S i) n b'
+  end.
+
+Definition boundaries := build_boundaries_from O 160 B0.
+
+Definition boundary i := nth i boundaries B0.
+
+Lemma boundary0:
+  boundary O = B0.
+Proof.
+  reflexivity.
+Qed.
+
+Definition pair_default : DH0*DH0 := ((A,[]),(A,[])).
+
+Definition pair_of_tokens a b :=
+  match a,b with
+  | RTok qR, LTok qL => ((qR,[]),(qL,[]))
+  | _, _ => pair_default
+  end.
+
+Definition pair_at b k :=
+  pair_of_tokens (tok_at b (k*2)) (tok_at b (S (k*2))).
+
+Fixpoint pair_list b off len :=
+  match len with
+  | O => []
+  | S len => pair_at b off :: pair_list b (S off) len
+  end.
+
+CoFixpoint pair_stream_from b off : Stream (DH0*DH0) :=
+  Cons (pair_at b off) (pair_stream_from b (S off)).
+
+Definition pair_pre_len b := (b.(b_mu) + 1) / 2.
+Definition pair_per_len b := b.(b_p) / 2.
+
+Definition row_table : list (nat*nat*nat*nat*nat*nat) :=
+  [(1,16,24,21,24,18); (2,24,18,20,18,22); (3,18,20,21,22,20);
+   (4,18,14,23,20,26); (5,16,22,22,26,18); (6,22,20,15,18,12);
+   (7,18,14,5,4,6); (8,14,10,21,24,18); (9,10,10,20,18,22);
+   (10,7466,6792,21,22,20); (11,6792,8836,23,20,26); (12,8834,6122,22,26,18);
+   (13,6254,4174,15,18,12); (14,4172,6248,5,4,6); (15,6248,4678,21,24,18);
+   (16,4678,5722,20,18,22); (17,5722,5208,21,22,20); (18,5206,6726,23,20,26);
+   (19,6724,4660,22,26,18); (20,4792,3228,15,18,12); (21,3226,4794,5,4,6);
+   (22,4794,3606,21,24,18); (23,3606,4378,20,18,22); (24,4378,3968,21,22,20);
+   (25,3966,5126,23,20,26); (26,5124,3552,22,26,18); (27,3552,2408,15,18,12);
+   (28,2408,3540,5,4,6); (29,3540,2676,21,24,18); (30,2674,3242,20,18,22);
+   (31,3240,2948,21,22,20); (32,2948,3744,23,20,26); (33,3744,2630,22,26,18);
+   (34,2630,1866,15,18,12); (35,1868,2616,5,4,6); (36,2616,2024,21,24,18);
+   (37,2024,2348,20,18,22); (38,2718,2434,21,22,20); (39,2434,3132,23,20,26);
+   (40,3130,2200,22,26,18); (41,2200,1576,15,18,12); (42,1576,2178,5,4,6);
+   (43,2178,1680,21,24,18); (44,1678,2026,20,18,22); (45,2104,1880,21,22,20);
+   (46,1880,2356,23,20,26); (47,2354,1684,22,26,18); (48,1684,1228,15,18,12);
+   (49,1228,1714,5,4,6); (50,1714,1346,21,24,18); (51,1344,1518,20,18,22);
+   (52,1528,1386,21,22,20); (53,1386,1714,23,20,26); (54,1712,1242,22,26,18);
+   (55,1242,944,15,18,12); (56,944,1212,5,4,6); (57,1212,934,21,24,18);
+   (58,932,1082,20,18,22); (59,1080,974,21,22,20); (60,974,1176,23,20,26);
+   (61,1176,868,22,26,18); (62,868,688,15,18,12); (63,690,860,5,4,6);
+   (64,860,700,21,24,18); (65,698,760,20,18,22); (66,1146,1034,21,22,20);
+   (67,1034,1272,23,20,26); (68,1270,920,22,26,18); (69,920,710,15,18,12);
+   (70,710,910,5,4,6); (71,910,758,21,24,18); (72,756,846,20,18,22);
+   (73,844,750,21,22,20); (74,750,888,23,20,26); (75,888,670,22,26,18);
+   (76,670,550,15,18,12); (77,552,676,5,4,6); (78,676,554,21,24,18);
+   (79,554,600,20,18,22); (80,600,524,21,22,20); (81,522,628,23,20,26);
+   (82,628,450,22,26,18); (83,454,384,15,18,12); (84,382,448,5,4,6);
+   (85,448,376,21,24,18); (86,376,414,20,18,22); (87,544,482,21,22,20);
+   (88,482,576,23,20,26); (89,574,416,22,26,18); (90,416,346,15,18,12);
+   (91,346,404,5,4,6); (92,404,326,21,24,18); (93,324,340,20,18,22);
+   (94,338,286,21,22,20); (95,286,332,23,20,26); (96,332,262,22,26,18);
+   (97,262,264,15,18,12); (98,266,270,5,4,6); (99,270,226,21,24,18);
+   (100,226,222,20,18,22); (101,242,200,21,22,20); (102,200,254,23,20,26);
+   (103,252,202,22,26,18); (104,202,176,15,18,12); (105,176,162,5,4,6);
+   (106,162,150,21,24,18); (107,148,142,20,18,22); (108,140,124,21,22,20);
+   (109,124,114,23,20,26); (110,114,84,22,26,18); (111,84,98,15,18,12);
+   (112,100,84,5,4,6); (113,84,84,21,24,18); (114,82,84,20,18,22);
+   (115,82,80,21,22,20); (116,80,70,23,20,26); (117,70,64,22,26,18);
+   (118,62,62,15,18,12); (119,64,74,5,4,6); (120,74,64,21,24,18);
+   (121,62,72,20,18,22); (122,70,62,21,22,20); (123,62,48,23,20,26);
+   (124,48,54,22,26,18); (125,52,46,15,18,12); (126,48,52,5,4,6);
+   (127,52,52,21,24,18); (128,50,50,20,18,22); (129,48,40,21,22,20);
+   (130,40,32,23,20,26); (131,32,30,22,26,18); (132,46,42,15,18,12);
+   (133,40,42,5,4,6); (134,42,32,21,24,18); (135,32,38,20,18,22);
+   (136,38,26,21,22,20); (137,24,18,23,20,26); (138,16,20,22,26,18);
+   (139,20,14,15,18,12); (140,14,18,5,4,6); (141,28,22,21,24,18);
+   (142,22,22,20,18,22); (143,20,20,21,22,20); (144,20,14,23,20,26);
+   (145,14,18,22,26,18); (146,18,12,15,18,12); (147,12,10,5,4,6);
+   (148,10,10,21,24,18); (149,10,6,20,18,22); (150,6,4,21,22,20);
+   (151,2,O,23,20,26); (152,O,O,22,26,18); (153,22,18,15,18,12);
+   (154,16,24,5,4,6); (155,24,18,21,24,18); (156,18,20,20,18,22);
+   (157,20,14,21,22,20); (158,12,10,23,20,26); (159,8,8,22,26,18);
+   (160,14,12,15,18,12); (147,10,10,5,4,6)].
+
+Definition row_at i := nth i row_table (S i,O,O,O,O,O).
+
+Definition seg_bound := 10000.
+
+Definition row_cert_at i addL addR w :=
+  let '(j,l0,r0,_vis,dL,dR) := row_at i in
+  let bL := boundary i in
+  let bR := boundary j in
+  let offL := l0 / 2 + addL in
+  let offR := r0 / 2 + addR in
+  let lenL := dL / 2 in
+  let lenR := dR / 2 in
+  andb (pair_pre_len bL <=? offL)
+  (andb (pair_pre_len bR <=? offR)
+  (andb (0 <? lenL)
+  (andb (0 <? lenR)
+  (andb (0 <? pair_per_len bL)
+  (andb (0 <? pair_per_len bR)
+  (andb (bL.(b_p) mod 2 =? 0)
+  (andb (bR.(b_p) mod 2 =? 0)
+  (andb (lenL mod pair_per_len bL =? 0)
+  (andb (lenR mod pair_per_len bR =? 0)
+  (andb
+    (segRLs_n1_c tm (pair_list bL O offL) (pair_list bR O offR) [S0] w seg_bound)
+    (segRLs_n1_c tm (pair_list bL offL lenL) (pair_list bR offR lenR) w w seg_bound))))))))))).
+
+Definition row_choices : list (nat*nat*list Sym) :=
+  [(0,0,[S0]); (0,0,[S1]); (0,1,[S0]); (0,1,[S1]);
+   (1,0,[S0]); (1,0,[S1]); (1,1,[S0]); (1,1,[S1])].
+
+Fixpoint find_row_choice i choices :=
+  match choices with
+  | [] => None
+  | (addL,addR,w)::choices =>
+      if row_cert_at i addL addR w then Some (addL,addR,w)
+      else find_row_choice i choices
+  end.
+
+Definition row_choice i := find_row_choice i row_choices.
+
+Definition row_cert i :=
+  match row_choice i with
+  | Some _ => true
+  | None => false
+  end.
+
+Definition rows_ok := forallb row_cert (seq 0 161).
+
+Lemma rows_ok_true:
+  rows_ok = true.
+Proof.
+  native_compute.
+  reflexivity.
+Qed.
+
+Lemma forallb_in {A} (f : A -> bool) x xs:
+  forallb f xs = true ->
+  In x xs ->
+  f x = true.
+Proof.
+  induction xs as [|y ys IH]; cbn.
+  - contradiction.
+  - intros H Hin.
+    apply andb_true_iff in H as [Hy Hys].
+    destruct Hin as [Heq|Hin].
+    + subst.
+      exact Hy.
+    + eapply IH; eauto.
+Qed.
+
+Lemma find_row_choice_spec i choices addL addR w:
+  find_row_choice i choices = Some (addL,addR,w) ->
+  row_cert_at i addL addR w = true.
+Proof.
+  induction choices as [|[[addL0 addR0] w0] choices IH]; cbn.
+  - congruence.
+  - destruct (row_cert_at i addL0 addR0 w0) eqn:Hcert.
+    + intro H.
+      inversion H; subst.
+      exact Hcert.
+    + apply IH.
+Qed.
+
+Lemma row_choice_spec i addL addR w:
+  row_choice i = Some (addL,addR,w) ->
+  row_cert_at i addL addR w = true.
+Proof.
+  apply find_row_choice_spec.
+Qed.
+
+Opaque row_choice.
+
+Definition row_target i := let '(j,_,_,_,_,_) := row_at i in j.
+Definition row_L0 i := let '(_,l0,_,_,_,_) := row_at i in l0.
+Definition row_R0 i := let '(_,_,r0,_,_,_) := row_at i in r0.
+Definition row_dL i := let '(_,_,_,_,dL,_) := row_at i in dL.
+Definition row_dR i := let '(_,_,_,_,_,dR) := row_at i in dR.
+
+Definition src_off i add := row_L0 i / 2 + add.
+Definition tgt_off i add := row_R0 i / 2 + add.
+Definition src_len i := row_dL i / 2.
+Definition tgt_len i := row_dR i / 2.
+
+Definition src_prefix i add := pair_list (boundary i) O (src_off i add).
+Definition tgt_prefix i add := pair_list (boundary (row_target i)) O (tgt_off i add).
+Definition src_loop i add := pair_list (boundary i) (src_off i add) (src_len i).
+Definition tgt_loop i add := pair_list (boundary (row_target i)) (tgt_off i add) (tgt_len i).
+
+Definition true_boundary_stream i := pair_stream_from (boundary i) O.
+
+Lemma pair_list_length b off len:
+  List.length (pair_list b off len) = len.
+Proof.
+  revert off.
+  induction len; intros off; cbn.
+  - reflexivity.
+  - rewrite IHlen.
+    reflexivity.
+Qed.
+
+Lemma pair_stream_split b off len:
+  pair_stream_from b off =
+  pair_list b off len *> pair_stream_from b (off + len).
+Proof.
+  revert off.
+  induction len; intros off; cbn.
+  - replace (off + 0) with off by lia.
+    reflexivity.
+  - rewrite Cons_unfold at 1.
+    cbn.
+    rewrite IHlen.
+    replace (S off + len) with (off + S len) by lia.
+    reflexivity.
+Qed.
+
+Lemma pair_pre_len_bound b k:
+  pair_pre_len b <= k ->
+  b.(b_mu) <= k*2.
+Proof.
+  unfold pair_pre_len.
+  lia.
+Qed.
+
+Lemma pair_period_double b:
+  b.(b_p) mod 2 = 0 ->
+  b.(b_p) = pair_per_len b * 2.
+Proof.
+  unfold pair_per_len.
+  intro Hmod.
+  pose proof (Nat.div_mod b.(b_p) 2 ltac:(lia)) as Hdiv.
+  lia.
+Qed.
+
+Lemma period_shift_mod p per len k:
+  p = per*2 ->
+  per <> O ->
+  len mod per = O ->
+  ((k*len)*2) mod p = O.
+Proof.
+  intros Hp Hper Hmod.
+  subst p.
+  apply Nat.mod_divide; [lia|].
+  apply Nat.mod_divide in Hmod; [|assumption].
+  destruct Hmod as [q Hq].
+  exists (k*q).
+  nia.
+Qed.
+
+Lemma tok_at_period_mod b n d:
+  b.(b_mu) <= n ->
+  b.(b_p) <> O ->
+  d mod b.(b_p) = O ->
+  tok_at b (n+d) = tok_at b n.
+Proof.
+  intros Hmu Hp Hmod.
+  unfold tok_at.
+  destruct (n <? b.(b_mu)) eqn:Hn.
+  - apply Nat.ltb_lt in Hn.
+    lia.
+  - destruct (n+d <? b.(b_mu)) eqn:Hnd.
+    + apply Nat.ltb_lt in Hnd.
+      lia.
+    + f_equal.
+      replace (n+d-b.(b_mu)) with (n-b.(b_mu)+d) by lia.
+      rewrite Nat.add_mod by exact Hp.
+      rewrite Hmod, Nat.add_0_r.
+      rewrite Nat.mod_mod by exact Hp.
+      reflexivity.
+Qed.
+
+Lemma pair_at_period_mod b k shift:
+  pair_pre_len b <= k ->
+  b.(b_p) <> O ->
+  (shift*2) mod b.(b_p) = O ->
+  pair_at b (k+shift) = pair_at b k.
+Proof.
+  intros Hpre Hp Hmod.
+  unfold pair_at.
+  f_equal.
+  - replace ((k+shift)*2) with (k*2+shift*2) by lia.
+    apply tok_at_period_mod; auto.
+    eapply pair_pre_len_bound.
+    exact Hpre.
+  - replace (S ((k+shift)*2)) with (S (k*2)+shift*2) by lia.
+    apply tok_at_period_mod; auto.
+    pose proof (pair_pre_len_bound b k Hpre).
+    lia.
+Qed.
+
+Lemma pair_list_period_shift b off len shift:
+  pair_pre_len b <= off ->
+  b.(b_p) <> O ->
+  (shift*2) mod b.(b_p) = O ->
+  pair_list b (off+shift) len = pair_list b off len.
+Proof.
+  revert off.
+  induction len; intros off Hpre Hp Hmod; cbn.
+  - reflexivity.
+  - rewrite (pair_at_period_mod b off shift Hpre Hp Hmod).
+    f_equal.
+    replace (S (off+shift)) with (S off+shift) by lia.
+    apply IHlen; auto.
+Qed.
+
+Lemma pair_list_period_repeat b off len k:
+  pair_pre_len b <= off ->
+  b.(b_p) = pair_per_len b*2 ->
+  pair_per_len b <> O ->
+  len mod pair_per_len b = O ->
+  pair_list b (off+k*len) len = pair_list b off len.
+Proof.
+  intros Hpre Hp Hper Hmod.
+  apply pair_list_period_shift; auto.
+  - lia.
+  - eapply period_shift_mod; eauto.
+Qed.
+
+Lemma row_cert_at_prefix_seg i addL addR w:
+  row_cert_at i addL addR w = true ->
+  segRLs_n tm (src_prefix i addL) (tgt_prefix i addR) [S0] w 1.
+Proof.
+  unfold row_cert_at, src_prefix, tgt_prefix, src_off, tgt_off,
+    row_L0, row_R0, row_dL, row_dR, row_target.
+  destruct (row_at i) as [[[[[j l0] r0] vis] dL] dR].
+  cbv beta iota zeta.
+  intro H.
+  apply andb_true_iff in H as [_ H].
+  apply andb_true_iff in H as [_ H].
+  apply andb_true_iff in H as [_ H].
+  apply andb_true_iff in H as [_ H].
+  apply andb_true_iff in H as [_ H].
+  apply andb_true_iff in H as [_ H].
+  apply andb_true_iff in H as [_ H].
+  apply andb_true_iff in H as [_ H].
+  apply andb_true_iff in H as [_ H].
+  apply andb_true_iff in H as [_ H].
+  apply andb_true_iff in H as [Hprefix _].
+  eapply segRLs_n1_c_spec.
+  exact Hprefix.
+Qed.
+
+Lemma row_cert_at_loop_seg i addL addR w:
+  row_cert_at i addL addR w = true ->
+  segRLs_n tm (src_loop i addL) (tgt_loop i addR) w w 1.
+Proof.
+  unfold row_cert_at, src_loop, tgt_loop, src_off, tgt_off, src_len, tgt_len,
+    row_L0, row_R0, row_dL, row_dR, row_target.
+  destruct (row_at i) as [[[[[j l0] r0] vis] dL] dR].
+  cbv beta iota zeta.
+  intro H.
+  apply andb_true_iff in H as [_ H].
+  apply andb_true_iff in H as [_ H].
+  apply andb_true_iff in H as [_ H].
+  apply andb_true_iff in H as [_ H].
+  apply andb_true_iff in H as [_ H].
+  apply andb_true_iff in H as [_ H].
+  apply andb_true_iff in H as [_ H].
+  apply andb_true_iff in H as [_ H].
+  apply andb_true_iff in H as [_ H].
+  apply andb_true_iff in H as [_ H].
+  apply andb_true_iff in H as [_ Hloop].
+  eapply segRLs_n1_c_spec.
+  exact Hloop.
+Qed.
+
+Lemma row_cert_at_params i addL addR w:
+  row_cert_at i addL addR w = true ->
+  pair_pre_len (boundary i) <= src_off i addL /\
+  pair_pre_len (boundary (row_target i)) <= tgt_off i addR /\
+  O < src_len i /\
+  O < tgt_len i /\
+  pair_per_len (boundary i) <> O /\
+  pair_per_len (boundary (row_target i)) <> O /\
+  (boundary i).(b_p) = pair_per_len (boundary i)*2 /\
+  (boundary (row_target i)).(b_p) =
+    pair_per_len (boundary (row_target i))*2 /\
+  src_len i mod pair_per_len (boundary i) = O /\
+  tgt_len i mod pair_per_len (boundary (row_target i)) = O.
+Proof.
+  unfold row_cert_at, src_off, tgt_off, src_len, tgt_len,
+    row_L0, row_R0, row_dL, row_dR, row_target.
+  destruct (row_at i) as [[[[[j l0] r0] vis] dL] dR].
+  cbv beta iota zeta.
+  intro H.
+  apply andb_true_iff in H as [HpreL H].
+  apply andb_true_iff in H as [HpreR H].
+  apply andb_true_iff in H as [HlenL H].
+  apply andb_true_iff in H as [HlenR H].
+  apply andb_true_iff in H as [HperL H].
+  apply andb_true_iff in H as [HperR H].
+  apply andb_true_iff in H as [HevenL H].
+  apply andb_true_iff in H as [HevenR H].
+  apply andb_true_iff in H as [HmodL H].
+  apply andb_true_iff in H as [HmodR _].
+  apply Nat.leb_le in HpreL.
+  apply Nat.leb_le in HpreR.
+  apply Nat.ltb_lt in HlenL.
+  apply Nat.ltb_lt in HlenR.
+  apply Nat.ltb_lt in HperL.
+  apply Nat.ltb_lt in HperR.
+  apply Nat.eqb_eq in HevenL.
+  apply Nat.eqb_eq in HevenR.
+  apply Nat.eqb_eq in HmodL.
+  apply Nat.eqb_eq in HmodR.
+  repeat split; try assumption; try lia.
+  - apply pair_period_double.
+    exact HevenL.
+  - apply pair_period_double.
+    exact HevenR.
+Qed.
+
+Lemma row_tail_downRect i addL addR w:
+  row_cert_at i addL addR w = true ->
+  downRect tm
+    (pair_stream_from (boundary i) (src_off i addL))
+    (pair_stream_from (boundary (row_target i)) (tgt_off i addR))
+    w 1.
+Proof.
+  intro Hcert.
+  destruct (row_cert_at_params i addL addR w Hcert)
+    as [HpreL [HpreR [HlenL [HlenR [HperL [HperR
+       [HpL [HpR [HmodL HmodR]]]]]]]]].
+  eapply segRLs_n_inf_trans with
+    (P := fun L R top => exists k,
+      L = pair_stream_from (boundary i) (src_off i addL + k*src_len i) /\
+      R = pair_stream_from (boundary (row_target i))
+            (tgt_off i addR + k*tgt_len i) /\
+      top = w).
+  - intros L R top [k [HL [HR Htop]]].
+    subst L R top.
+    exists
+      (pair_list (boundary i) (src_off i addL + k*src_len i) (src_len i)),
+      (pair_list (boundary (row_target i))
+        (tgt_off i addR + k*tgt_len i) (tgt_len i)),
+      w,
+      (pair_stream_from (boundary i)
+        (src_off i addL + k*src_len i + src_len i)),
+      (pair_stream_from (boundary (row_target i))
+        (tgt_off i addR + k*tgt_len i + tgt_len i)).
+    split.
+    + rewrite pair_list_length.
+      exact HlenR.
+    + split.
+      * rewrite (pair_stream_split (boundary i)
+          (src_off i addL + k*src_len i) (src_len i)).
+        reflexivity.
+      * split.
+        -- rewrite (pair_stream_split (boundary (row_target i))
+             (tgt_off i addR + k*tgt_len i) (tgt_len i)).
+           reflexivity.
+        -- split.
+           ++ rewrite (pair_list_period_repeat (boundary i)
+                (src_off i addL) (src_len i) k HpreL HpL HperL HmodL).
+              rewrite (pair_list_period_repeat (boundary (row_target i))
+                (tgt_off i addR) (tgt_len i) k HpreR HpR HperR HmodR).
+              eapply row_cert_at_loop_seg.
+              exact Hcert.
+           ++ exists (S k).
+              split.
+              {
+                replace (src_off i addL + S k*src_len i)
+                   with (src_off i addL + k*src_len i + src_len i) by lia.
+                reflexivity.
+              }
+              split.
+              {
+                replace (tgt_off i addR + S k*tgt_len i)
+                      with (tgt_off i addR + k*tgt_len i + tgt_len i) by lia.
+                reflexivity.
+              }
+              reflexivity.
+  - exists O.
+    split.
+    + replace (src_off i addL + O*src_len i) with (src_off i addL) by lia.
+      reflexivity.
+    + split.
+      * replace (tgt_off i addR + O*tgt_len i) with (tgt_off i addR) by lia.
+        reflexivity.
+      * reflexivity.
+Qed.
+
+Lemma row_downRect_from_cert i addL addR w:
+  row_cert_at i addL addR w = true ->
+  downRect tm
+    (true_boundary_stream i)
+    (true_boundary_stream (row_target i))
+    [S0] 1.
+Proof.
+  intro Hcert.
+  unfold true_boundary_stream.
+  rewrite (pair_stream_split (boundary i) O (src_off i addL)).
+  rewrite (pair_stream_split (boundary (row_target i)) O (tgt_off i addR)).
+  replace (O + src_off i addL) with (src_off i addL) by lia.
+  replace (O + tgt_off i addR) with (tgt_off i addR) by lia.
+  eapply segRLs_n_downRect_trans.
+  - eapply row_cert_at_prefix_seg.
+    exact Hcert.
+  - eapply row_tail_downRect.
+    exact Hcert.
+Qed.
+
+Definition row_target_member i :=
+  existsb (Nat.eqb (row_target i)) (seq O 161).
+
+Definition rows_target_ok :=
+  forallb row_target_member (seq O 161).
+
+Lemma rows_target_ok_true:
+  rows_target_ok = true.
+Proof.
+  native_compute.
+  reflexivity.
+Qed.
+
+Lemma row_target_in i:
+  In i (seq O 161) ->
+  In (row_target i) (seq O 161).
+Proof.
+  intro Hin.
+  pose proof rows_target_ok_true as Hok.
+  unfold rows_target_ok in Hok.
+  eapply forallb_in in Hok; [|exact Hin].
+  unfold row_target_member in Hok.
+  apply existsb_exists in Hok as [j [Hj Heq]].
+  apply Nat.eqb_eq in Heq.
+  subst j.
+  exact Hj.
+Qed.
+
+Lemma row_choice_some i:
+  In i (seq O 161) ->
+  exists addL addR w, row_choice i = Some (addL,addR,w).
+Proof.
+  intro Hin.
+  pose proof rows_ok_true as Hok.
+  unfold rows_ok in Hok.
+  eapply forallb_in in Hok; [|exact Hin].
+  unfold row_cert in Hok.
+  destruct (row_choice i) as [[[addL addR] w]|] eqn:Hchoice;
+    cbn in Hok; try discriminate.
+  exists addL, addR, w.
+  reflexivity.
+Qed.
+
+Lemma right_quadRect:
+  quadRect tm (true_boundary_stream O) (const S0).
+Proof.
+  eapply downRect_inf_concat with
+    (P := fun L top =>
+      exists i, In i (seq O 161) /\
+        L = true_boundary_stream i /\
+        top = const S0).
+  - intros L top [i [Hin [HL Htop]]].
+    subst L top.
+    destruct (row_choice_some i Hin) as [addL [addR [bot Hchoice]]].
+    pose proof (row_choice_spec i addL addR bot Hchoice) as Hcert.
+    exists (true_boundary_stream (row_target i)), (const S0), [S0], 1.
+    split; [lia|].
+    split.
+    + cbn; rewrite <- const_unfold; reflexivity.
+    + split.
+      * eapply row_downRect_from_cert.
+        exact Hcert.
+      * exists (row_target i).
+        split.
+        -- apply row_target_in.
+           exact Hin.
+        -- split; reflexivity.
+  - exists O.
+    split.
+    + cbn; auto.
+    + split; reflexivity.
+Qed.
+
+Fixpoint link_pairs (hs : list (DH0*DH0)) (h : DH0) : list (DH0*DH0) :=
+  match hs with
+  | [] => []
+  | p::rest =>
+      match rest with
+      | [] => [(snd p,h)]
+      | q::_ => (snd p,fst q)::link_pairs rest h
+      end
+  end.
+
+Definition left_start : DH0 := (E,[]).
+Definition left_loop_head : DH0 := (A,[]).
+Definition left_entry_side : side := [S0;S1;S1] *> const S0.
+Definition left_after n : side := ([S0;S0] ++ [S1]^^(9+n*2)) *> const S0.
+
+Definition left_prefix_pairs := pair_list B0 O 8.
+Definition left_loop_pairs := pair_list B0 8 3.
+Definition left_prefix_crossings :=
+  link_pairs left_prefix_pairs left_loop_head.
+Definition left_period :=
+  link_pairs left_loop_pairs left_loop_head.
+
+Lemma left_prefix_lcons:
+  lcons left_start left_prefix_crossings =
+  (left_prefix_pairs,left_loop_head).
+Proof.
+  native_compute.
+  reflexivity.
+Qed.
+
+Lemma left_loop_lcons:
+  lcons left_loop_head left_period =
+  (left_loop_pairs,left_loop_head).
+Proof.
+  native_compute.
+  reflexivity.
+Qed.
+
+Lemma left_prefix_side:
+  sideRLs (flip tm) left_prefix_crossings left_entry_side (left_after O).
+Proof.
+  eapply sideRLs_c_spec with (r' := left_after O) (T := 1000).
+  - native_compute.
+    reflexivity.
+  - reflexivity.
+Qed.
+
+Lemma left_period_side n:
+  sideRLs (flip tm) left_period (left_after n) (left_after (S n)).
+Proof.
+  unfold left_period, left_loop_pairs, left_loop_head, left_after, link_pairs.
+  cbn.
+  esx.
+Qed.
+
+Lemma B0_loop_split n:
+  pair_stream_from B0 (8+n*3) =
+  left_loop_pairs *> pair_stream_from B0 (8+S n*3).
+Proof.
+  rewrite (pair_stream_split B0 (8+n*3) 3).
+  replace (8+n*3+3) with (8+S n*3) by lia.
+  unfold left_loop_pairs.
+  rewrite (pair_list_period_repeat B0 8 3 n).
+  - reflexivity.
+  - native_compute.
+    lia.
+  - native_compute.
+    reflexivity.
+  - native_compute.
+    lia.
+  - native_compute.
+    reflexivity.
+Qed.
+
+Lemma left_tail_realizes:
+  leftRealizes tm left_loop_head (pair_stream_from B0 8) (left_after O).
+Proof.
+  eapply leftRealizes_inf_concat with
+    (P := fun h L l =>
+      exists n, h = left_loop_head /\
+        L = pair_stream_from B0 (8+n*3) /\
+        l = left_after n).
+  - intros h L l [n [Hh [HL Hl]]].
+    subst h L l.
+    exists left_loop_pairs,
+      (pair_stream_from B0 (8+S n*3)),
+      left_loop_head,
+      left_period,
+      (left_after (S n)).
+    split.
+    + native_compute.
+      lia.
+    + split.
+      * apply B0_loop_split.
+      * split.
+        -- apply left_loop_lcons.
+        -- split.
+           ++ apply left_period_side.
+           ++ exists (S n).
+              repeat split; reflexivity.
+  - exists O.
+    repeat split; reflexivity.
+Qed.
+
+Lemma left_realizes:
+  leftRealizes tm left_start (true_boundary_stream O) left_entry_side.
+Proof.
+  unfold true_boundary_stream.
+  rewrite boundary0.
+  rewrite (pair_stream_split B0 O 8).
+  replace (O+8) with 8 by lia.
+  eapply sideRLs_leftRealizes_trans.
+  - apply left_prefix_lcons.
+  - apply left_prefix_side.
+  - apply left_tail_realizes.
+Qed.
+
+Lemma entry_progress:
+  c0 -[ tm ]->+ left_entry_side {{{ (left_start,R) }}} const S0.
+Proof.
+  unfold left_entry_side, left_start.
+  execute.
+Qed.
+
+Lemma entry_nonhalt:
+  ~halts tm (left_entry_side {{{ (left_start,R) }}} const S0).
+Proof.
+  eapply quadRect_nonhalt.
+  - apply right_quadRect.
+  - apply left_realizes.
+Qed.
+
+Lemma nonhalt:
+  ~halts tm c0.
+Proof.
+  eapply multistep_nonhalt.
+  - apply progress_evstep.
+    apply entry_progress.
+  - apply entry_nonhalt.
+Qed.
+
+End TM4.
